Graph_Inversion.thy
@@ -1,5 +1,5 @@
 theory Graph_Inversion
-imports GraphUtils
+imports GraphUtils Refine_Monadic.Refine_Monadic
 begin
 
 definition invert_graph :: "_ graph \<Rightarrow> _ graph" (*("(_\<inverse>)" [1000] 999)*) where
@@ -12,6 +12,9 @@ abbreviation (input) invert_syntax (infix "\<up>" 55)
 
 lemma invert_invert[simp]: "invert_graph (invert_graph c) = c"
   unfolding invert_graph_def by fastforce
+
+lemma invert_concrete: "(invert_graph c) (u, v) = c (v, u)"
+  unfolding invert_graph_def by simp
 
 lemma invert_E: "Graph.E (invert_graph c) = (Graph.E c)\<inverse>"
   unfolding Graph.E_def invert_graph_def by auto
@@ -87,6 +90,7 @@ lemma invert_min_dist:
 text \<open>The following lemmas relate properties of the inverted graph to the corresponding ones in the
       non-inverted graph.\<close>
 lemmas invert_graph_simps[simp] =
+  invert_concrete
   invert_E
   invert_V
   invert_incoming
@@ -104,4 +108,67 @@ lemmas invert_graph_simps[simp] =
   invert_dist
   invert_min_dist
 
+subsection \<open>Refinement setup\<close>
+
+thm conc_fun_chain
+term conc_fun
+term single_valued
+find_theorems single_valued
+thm br_sv
+term br
+thm br_def
+thm galois_connection_def
+find_theorems "_ = (\<lambda>_. True)"
+thm Option.Option.option.pred_True
+find_consts "_ \<Rightarrow> bool" name:True
+thm Quot_True_def
+term Quot_True
+find_theorems single_valued "(\<Down>)"
+thm conc_abs_swap
+
+(* TODO how to express this more elegantly *)
+definition invert_graph_rel :: "(_ graph) rel" where
+  "invert_graph_rel \<equiv> {(c, invert_graph c) | c. True}"
+
+lemma invert_graph_rel_alt: "invert_graph_rel = br invert_graph (\<lambda>_. True)"
+  unfolding invert_graph_rel_def br_def by blast
+
+lemma invert_graph_rel_sv: "single_valued invert_graph_rel"
+  unfolding invert_graph_rel_alt by (rule br_sv)
+
+lemma invert_graph_rel_comp[simp]: "invert_graph_rel O invert_graph_rel = Id"
+  unfolding invert_graph_rel_def by fastforce
+
+(* TODO improve or remove *)
+thm Id_refine conc_abs_swap conc_fun_chain dual_order.eq_iff dual_order.refl dual_order.trans invert_graph_rel_comp invert_graph_rel_sv refine_IdD
+lemma "\<Up> invert_graph_rel = \<Down> invert_graph_rel"
+  apply (intro antisym)
+   apply (metis Id_refine conc_abs_swap conc_fun_chain invert_graph_rel_comp invert_graph_rel_sv le_funI)
+  by (metis (no_types, lifting) Id_refine conc_Id conc_abs_swap conc_fun_chain conc_trans id_apply invert_graph_rel_comp invert_graph_rel_sv le_funI)
+  (*by (metis Id_refine conc_abs_swap conc_fun_chain dual_order.eq_iff dual_order.refl dual_order.trans invert_graph_rel_comp invert_graph_rel_sv refine_IdD)*)
+
+locale Dual_Graph_Algorithms =
+  fixes alg alg' :: "_ graph \<Rightarrow> _ graph nres"
+  assumes dual_alg: "\<And>c. alg c = \<Down> invert_graph_rel (alg' (invert_graph c))"
+begin
+lemma dual_alg': "\<And>c. alg' c = \<Down> invert_graph_rel (alg (invert_graph c))"
+  using dual_alg by (simp add: conc_fun_chain)
+end
+
+(* TODO can it be sufficient to only show one direction? *)
+lemma Dual_Graph_AlgorithmsI[intro]:
+  assumes LE1: "\<And>c. alg c \<le> \<Down> invert_graph_rel (alg' (invert_graph c))"
+    and LE2: "\<And>c. alg' c \<le> \<Down> invert_graph_rel (alg (invert_graph c))"
+  shows "Dual_Graph_Algorithms alg alg'"
+proof (unfold_locales, intro antisym)
+  from LE1 show "\<And>c. alg c \<le> \<Down> invert_graph_rel (alg' (invert_graph c))" .
+  from LE2 show "\<And>c. \<Down> invert_graph_rel (alg' (invert_graph c)) \<le> alg c"
+    by (metis (no_types, lifting) conc_Id conc_fun_chain conc_trans dual_order.refl id_apply invert_graph_rel_comp invert_invert)
+qed
+
+(* TODO sanity check *)
+lemma
+  assumes "\<And>c. alg c \<le> \<Down> invert_graph_rel (alg' (invert_graph c))"
+  shows "\<And>c. alg' c \<le> \<Down> invert_graph_rel (alg (invert_graph c))"
+  using assms oops
 end
